veric/SeparationLogicSoundness.v
@@ -88,7 +88,6 @@ Definition semax_ff := semax_ff Hspec.
 Definition semax1 := semax1 Hspec.
 Definition function_body_entry_assert  := function_body_entry_assert .
 Definition function_body_ret_assert  := function_body_ret_assert .
-Definition funsig := funsig.
 Definition fn_funsig := fn_funsig.
 Definition semax_external ef A P Q := forall n, semax_ext ef A P Q n.
 Definition for1_ret_assert := for1_ret_assert .
