veric/compcert_rmaps.v
@@ -4,8 +4,6 @@ Require Import veric.Address.
 Require Import veric.rmaps.
 Require Import veric.rmaps_lemmas.
 
-Definition funsig := (typelist * type)%type. (* argument and result signature *)
-
 Inductive kind : Type := VAL : memval -> kind 
                                    | LK : Z -> kind 
                                    | CT: Z -> kind 
